\baselineskip=15pt
$$
\halign{$# = {}$&\quad\hfil$#$\hfil&\qquad$#$&\quad\hfil$#$\hfil\cr
x^1 &x^{\underline 1} &=& x^{\overline 1}\cr
x^2 &x^{\underline 2} + x^{\underline 1} &=&x^{\overline 2} - x^{\overline 1} \cr
x^3 &x^{\underline 3} + 3 x^{\underline 2} + x^{\underline 1}
&=&x^{\overline 3}- 3 x^{\overline 2} + x^{\overline 1} \cr
x^4 &x^{\underline 4} + 6 x^{\underline 3}+ 7 x^{\underline 2} + x^{\underline 1}
 &=&x^{\overline 4} - 6 x^{\overline 3}+ 7 x^{\overline 2} - x^{\overline 1} \cr
x^5 &x^{\underline 5} + 15x^{\underline 4} + 25 x^{\underline 3}+ 10 x^{\underline 2} + x^{\underline 1}
 &=&x^{\underline 5} - 15 x^{\overline 4} + 25 x^{\overline 3}- 10 x^{\overline 2} + x^{\overline 1} \cr
\noalign{\vskip 8pt}
x^{\overline 1} &x^1 &x^{\underline 1} = {}&x^1\cr
x^{\overline 2} &x^2 + x^1&x^{\underline 2}= {}&x^2 - x^1\cr
x^{\overline 3}&x^3 + 3x^2 + 2x^1&x^{\underline 3}= {}&x^3 - 3x^2 + 2x^1\cr
x^{\overline 4}&x^4 + 6x^3 + 11x^2 + 6x^1&x^{\underline 4}= {}&x^4 - 6x^3 + 11x^2 - 6x^1\cr
x^{\overline 5}&x^5 + 10 x^4 + 35 x^3 + 50 x^2 + 24 x^1&x^{\underline 5}= {}& x^5 - 10 x^4 + 35 x^3 - 50 x^2 + 24 x^1\cr
}
$$
