Master method:
$$T(n) = aT(n/b) + f(n), \quad a\geq 1, b > 1$$
If $\exists \epsilon > 0$ such that $f(n) = O(n^{\log_b a - \epsilon})$ then
$$T(n) = \Theta(n^{\log_b a}).$$
\par
If $f(n) = \Theta(n^{\log_b a})$ then
$$T(n) = \Theta(n^{\log_b a} \log_2 n).$$
\par
If $\exists \epsilon > 0$ such that $f(n) = \Omega(n^{\log_b a + \epsilon})$,
and $\exists c < 1$ such that $a f(n/b) \leq cf(n)$ for large $n$,
then
$$T(n) = \Theta(f(n)).$$
\par
%\vskip 0.10in
Substitution (example): Consider the following recurrence
$$T_{i+1} = 2^{2^i} \cdot T_i^2, \quad T_1 = 2.$$
Note that $T_i$ is always a power of two.
Let $t_i = \log_2 T_i$.
Then we have
$$
t_{i+1} = 2^i + 2 t_i, \quad t_1 = 1.
$$
Let $u_i = t_i/2^i$.
Dividing both sides of the previous equation by $2^{i+1}$ we get
$$
{t_{i+1} \over 2^{i+1}} = {2^i \over 2^{i+1}} + {t_i \over 2^i}.
$$
Substituting we find
$$
u_{i+1} = \sfrac 1 2 + u_i, \qquad u_1 = \sfrac 1 2 ,
$$
which is simply $u_i = i/2$.
So we find that $T_i$ has the closed form $T_i = 2^{i2^{i-1}}$.
%\vskip 1em
\par
Summing factors (example): Consider the following recurrence
$$T(n) = 3T(n/2) + n, \quad T(1) = 1.$$
Rewrite so that all terms involving $T$ are on the
left side
$$T(n) - 3T(n/2) = n.$$
Now expand the recurrence,
and choose a factor which makes the left side ``telescope''
