Generating functions:
\halign{\quad#\hfil&\vtop{\parindent=0pt\hsize=2.0in\strut#\strut}\cr
1. &Multiply both sides of the equation by $x^i$. \cr
2. &Sum both sides over all $i$ for which the equation is valid. \cr
3. &Choose a generating function $G(x)$.
Usually $G(x) = \sum_{i=0}^\infty x^i g_i$.\cr
3. &Rewrite the equation in terms of the generating function $G(x)$. \cr
4. &Solve for $G(x)$. \cr
5. &The coefficient of $x^i$ in $G(x)$ is $g_i$.\cr
%6. &Check the answer! \cr
}
Example:
$$
g_{i+1} = 2 g_i + 1, \quad g_0 = 0.
$$
Multiply and sum:
$$
\sum_{i\geq 0} g_{i+1} x^i = \sum_{i\geq 0} 2 g_i x^i + \sum_{i\geq 0} x^i.
$$
We choose $G(x) = \sum_{i\geq 0} x^i g_i$.
Rewrite in terms of $G(x)$:
$$
{G(x) - g_0 \over x} = 2 G(x) + \sum_{i\geq 0} x^i.
$$
Simplify:
$$
{G(x) \over x} = 2 G(x) + {1 \over 1 -x}.
$$
Solve for $G(x)$:
$$
G(x) =  {x \over (1 -x)(1-2x)}.
$$
Expand this using partial fractions:
$$
\eqalign{
G(x) &= x \left( {2 \over 1 -2x} - {1 \over 1 - x}\right) \cr
&= x \left( 2 \sum_{i\geq 0} 2^i x^i - \sum_{i\geq 0} x^i\right) \cr
&= \sum_{i\geq 0} (2^{i+1} - 1) x^{i+1}.\cr
}
$$
So $g_i = 2^i - 1$.
%Plugging in some small values,
%this is confirmed.
