$$
\eqalign{
1 &\big(T(n) - 3T(n/2) = n\big) \cr
3 &\big(T(n/2) - 3T(n/4) = n/2\big) \cr
&\vdots  \qquad \vdots \qquad \vdots\cr
3^{\log_2 n - 1} &\big(T(2) - 3T(1) = 2\big) \cr
}$$
Let $m = \log_2 n$.
Summing the left side we get $T(n) - 3^mT(1) = T(n) - 3^m =  T(n) - n^k$ where $k = \log_2 3 \approx 1.58496$.
Summing the right side we get
$$
\sum_{i=0}^{m-1} {n \over 2^i} 3^i = n \sum_{i=0}^{m-1} \left(\sfrac 3 2 \right)^i.
$$
Let $c = {3 \over 2}$.
Then we have
$$
\eqalign{
n \sum_{i=0}^{m-1} c^i &= n \left( {c^m - 1 \over c - 1} \right) \cr
&= 2 n ( c^{\log_2 n } - 1 ) \cr
&= 2 n ( c^{(k-1) \log_c n } - 1 ) \cr
&= 2 n^k  - 2n, \cr
}$$
and so $T(n) = 3 n^k - 2n$.
Full history recurrences can often be changed to limited history ones (example):
Consider
$$T_i = 1 + \sum^{i-1}_{j=0} T_j, \quad T_0 = 1.$$
Note that
$$T_{i+1} = 1 + \sum^i_{j=0} T_j.$$
Subtracting we find
$$
\eqalign{
T_{i+1} - T_i &= 1 + \sum^i_{j=0} T_j - 1 - \sum^{i-1}_{j=0} T_j \cr
&= T_i. \cr
}$$
And so $T_{i+1} = 2T_i = 2^{i+1}$.
