\halign{\hfil$\displaystyle#$\hfil&\quad$\displaystyle#$\hfil\vadjust{\kern3pt}\cr
\hskip 1.09in &\hskip 1.15in \cr
\zeta(x) &{} = \prod_p {1 \over 1 - p^{-x}},\cr
\zeta^2(x) &{} = \sum_{i=1}^\infty {d(i) \over x^i} \quad \hbox{where $d(n) = \sum_{d \vert n} 1$},\hskip-0.02in\cr
\zeta(x)\zeta(x-1) &{} = \sum_{i=1}^\infty {S(i) \over x^i} \quad \hbox{where $S(n) = \sum_{d \vert n} d$},\hskip-0.06in\cr
\zeta(2n) &{} = {2^{2n-1} \vert B_{2n} \vert \over (2n)!} \pi^{2n}, \quad n \in \Natural,\cr
{x \over\sin x}
&{}= \sum_{i=0}^\infty (-1)^{i-1}{(4^i - 2) B_{2i} x^{2i} \over (2i)!},\cr
\left({1 - \sqrt{1-4x} \over 2x}\right)^n
&{}= \sum_{i=0}^\infty {n(2i + n - 1)! \over i! (n + i)!} x^i,\cr
e^x \sin x
&{}= \sum_{i=1}^\infty {2^{i/2} \sin \sfrac {i \pi} 4 \over i!} x^i,\cr
\sqrt{1 - \sqrt{1 -x} \over x}
&{}= \sum_{i=0}^\infty { (4i)! \over 16^i \sqrt{2} (2i)! (2i+1)!} x^i,\cr
\left({\arcsin x \over x}\right)^2
&{}= \sum_{i=0}^\infty { 4^i i!^2 \over (i + 1)(2i +1)!} x^{2i}.\cr
}
