Expansions:
\halign{\hfil$\displaystyle#$\hfil&\quad$\displaystyle#$\hfil&\quad\hfil$\displaystyle#$\hfil&\quad$\displaystyle#$\hfil\cr
{1 \over (1-x)^{n+1}}\ln{1 \over 1- x}
&{}= \sum_{i=0}^\infty (H_{n+i} - H_n) {n+i \choose i} x^i,
&\left({1 \over x}\right)^{\overline{-n}}
&{}= \sum_{i=0}^\infty \Subset i n x^i,\cr
x^{\overline{n}}
&{}= \sum_{i=0}^\infty \Cycle n i x^i,
&(e^x - 1)^n
&{}= \sum_{i=0}^\infty \Subset i n {n! x^i \over i!},\cr
\left(\ln {1 \over 1 -x}\right)^n
&{}= \sum_{i=0}^\infty \Cycle i n {n! x^i \over i!},
&x \cot x
&{}= \sum_{i=0}^\infty {(-4)^i B_{2i} x^{2i} \over (2i)!},\cr
\tan x
&{}= \sum_{i=1}^\infty (-1)^{i-1}{2^{2i} (2^{2i} - 1) B_{2i} x^{2i-1} \over (2i)!},
&\zeta(x)
&{}= \sum_{i=1}^\infty {1 \over i^x},\cr
{1 \over \zeta(x)}
&{}= \sum_{i=1}^\infty {\mu(i) \over i^x},
&{\zeta(x-1) \over \zeta(x)}
&{}= \sum_{i=1}^\infty {\phi(i) \over i^x},\cr
}
